#+TITLE: Lists :: Chapter 09
#+STARTUP: content

* Exercise: EnumFromTo
Page 306.

#+begin_src haskell
--
-- The "enum from to" functions return empty list if the starting
-- point is less than the ending point. Remember that sum (or) data
-- constructors behave like a number line. So, things to the left are
-- “less than” things on the right.
--
-- λ> :info Bool
-- data Bool = False | True
--
-- λ> enumFromTo True False
-- []
--
-- λ> enumFromTo False True
-- [False,True]
--
eftBool :: Bool -> Bool -> [Bool]
eftBool False _    = []
eftBool True False = [True, False]
eftBool _ _        = []

--
-- A very explicit and manual way of ranging over the tree possible
-- data constructors of `Ordering`.
--
eftOrd :: Ordering -> Ordering -> [Ordering]
eftOrd LT EQ = [LT, EQ]
eftOrd EQ LT = [EQ, LT]
eftOrd EQ GT = [EQ, GT]
eftOrd GT EQ = [GT, EQ]
eftOrd LT _  = [LT, EQ, GT]
eftOrd GT _  = [GT, EQ, LT]

--
-- Using recursion.
--
eftOrdering :: Ordering -> Ordering -> [Ordering]
eftOrdering ini end = run ini []
  where
    run current acc
          | (<) end current = []
          | (==) current end = (++) acc [current]
          | otherwise = run (succ current) ((++) acc [current])


--
-- ‘ini’ must be less than ‘end’. Does not handle randing down, or
-- negative values.
--
eftInt :: Int -> Int -> [Int]
eftInt ini end = go (ini + 1) [ini]
  where go current acc
          | end < current = []
          | current == end = acc ++ [current]
          | otherwise = go (current + 1) (acc ++ [current])


--
-- Only handles ranges “going up”.
--
eftChar :: Char -> Char -> [Char]
eftChar ini end = go (succ ini) [ini]
  where go current acc
          | end < current = []
          | current == end = acc ++ [current]
          | otherwise = go (succ current) (acc ++ [current])
#+end_src

* Exercises: Thy fearful symmetry
Page 310.

** 01
:PROPERTIES:
:CUSTOM_ID: section
:END:
#+begin_src haskell
myWords :: [Char] -> [[Char]]
myWords str = go str []
  where go s acc
          | s == "" = acc
          | head s == ' ' = go (tail s) acc
          | otherwise = go
                        (dropWhile (/= ' ') s)
                        (acc ++ [takeWhile (/= ' ') s])
--
-- [λ> myWords "Tomb Raider - The Angel Of Darkness"
-- ["Tomb","Raider","-","The","Angel","Of","Darkness"]
--
#+end_src

Another version:

#+begin_src haskell
{-# LANGUAGE NoMonomorphismRestriction #-}

dropWhileSpc :: [Char] -> [Char]
dropWhileSpc = dropWhile (== ' ')

dropUntilSpc :: [Char] -> [Char]
dropUntilSpc = dropWhile (/= ' ')

isSpc :: Char -> Bool
isSpc ' ' = True
isSpc _   = False

takeUntilSpc :: [Char] -> [Char]
takeUntilSpc = takeWhile (/= ' ')

toList :: a -> [a]
toList thing = (:) thing []

myWords :: [Char] -> [[Char]]
myWords s = go s []
  where
    go :: [Char] -> [[Char]] -> [[Char]]
    go xs acc
        | (==) xs [] = acc
        | isSpc . head $ xs = go (dropWhileSpc xs) acc
        | otherwise =
            go
              (dropUntilSpc xs)
              ((++) (toList . takeUntilSpc $ xs) acc)
--
-- λ> mapM_ putStrLn $ myWords "💖 Tomb Raider - Angel of Darkness 💯"
-- 💯
-- Darkness
-- of
-- Angel
-- -
-- Raider
-- Tomb
-- 💖
--
#+end_src

** 02

#+begin_src haskell
firstSen = "Tyger Tyger, burning bright\n"
secondSen = "In the forests of the night\n"
thirdSen = "What immortal hand or eye\n"
fourthSen = "Could frame thy fearful\
\ symmetry?"

sentences = firstSen ++ secondSen
            ++ thirdSen ++ fourthSen

shouldEqual =
  [ "Tyger Tyger, burning bright"
  , "In the forests of the night"
  , "What immortal hand or eye"
  , "Could frame thy fearful symmetry?"
  ]

dropUntilNL :: [Char] -> [Char]
dropUntilNL str
  | str == "" = str
  | head str == '\n' = tail str
  | otherwise = dropUntilNL (dropWhile (/= '\n') str)

myLines :: String -> [String]
myLines str = go str []
  where go s acc
          | s == "" = acc
          | otherwise = go (dropUntilNL s)
                           (acc ++ [takeWhile (/= '\n') s])

main :: IO ()
main = do
  print $
    "Are they equal? "
    ++ show (myLines sentences == shouldEqual)
#+end_src

** 03

#+begin_src haskell
firstSen = "Tyger Tyger, burning bright\n"
secondSen = "In the forests of the night\n"
thirdSen = "What immortal hand or eye\n"
fourthSen = "Could frame thy fearful\
\ symmetry?"

sentences :: [Char]
sentences = firstSen ++ secondSen
            ++ thirdSen ++ fourthSen

tombRaider :: [Char]
tombRaider = "Tomb Raider - The Angel of Darkness"

shouldEqualSentences :: [[Char]]
shouldEqualSentences =
  [ "Tyger Tyger, burning bright"
  , "In the forests of the night"
  , "What immortal hand or eye"
  , "Could frame thy fearful symmetry?"
  ]

shouldEqualTombRaider :: [[Char]]
shouldEqualTombRaider =
  [ "Tomb"
  , "Raider"
  , "-"
  , "The"
  , "Angel"
  , "of"
  , "Darkness"
  ]

dropUntil :: Char -> [Char] -> [Char]
dropUntil chr str
  | str == "" = str
  | head str == chr = tail str
  | otherwise = dropUntil chr (dropWhile (/= chr) str)

toList :: Char -> String -> [String]
toList chr str = go chr str []
  where go chr s acc
          | s == "" = acc
          | otherwise = go chr
                        (dropUntil chr s)
                        (acc ++ [takeWhile (/= chr) s])

main :: IO ()
main = do
  putStrLn $
    "Tomb Raider --: " ++
    (show $ toList ' ' tombRaider == shouldEqualTombRaider)

  putStrLn $
    "Sentences ----: " ++
    (show $ toList '\n' sentences == shouldEqualSentences)

--
-- λ> main
-- Tomb Raider --: True
-- Sentences ----: True
--
#+end_src

* Exercises: Comprehend thy lists
:PROPERTIES:
:CUSTOM_ID: exercises-comprehend-thy-lists
:END:
Page 314.

Required for the two exercises.

#+begin_example
λ> mySqr = [x ^ 2 | x <- [1..10]]
λ> mySqr
[1,4,9,16,25,36,49,64,81,100]
#+end_example

First exercise:

#+begin_example
λ> [x | x <- mySqr, rem x 2 == 0]
[4,16,36,64,100]
#+end_example

Second exercise:

#+begin_example
λ> [(x, y) | x <- mySqr,
            y <- mySqr,
            x < 50,
            y > 50]

λ> res
[(1,64),(1,81),(1,100),(4,64),(4,81),(4,100),(9,64),(9,81),(9,100),(16,64),(16,81),(16,100),(25,64),(25,81),(25,100),(36,64),(36,81),(36,100),(49,64),(49,81),(49,100)]
#+end_example

Combine each =x= with all =y=s. The =take 5= exercises just returns the
first 5 elements of the result above.

* Exercises: Square Cube
:PROPERTIES:
:CUSTOM_ID: exercises-square-cube
:END:
Page 316.

#+begin_src haskell
mySqr :: (Num a, Enum a) => [a]
mySqr = [x ^ 2 | x <- [1..5]]

myCube :: (Num a, Enum a) => [a]
myCube = [y ^ 3 | y <- [1..5]]

tup1 :: [(Integer, Integer)]
tup1 = [(x, y) | x <- mySqr, y <- myCube]

tup2 :: [(Integer, Integer)]
tup2 = [(x, y) | x <- mySqr,
                 y <- myCube,
                 x < 50,
                 y < 50]

qty :: Int
qty = length tup2
#+end_src

* Exercises: Bottom madness
:PROPERTIES:
:CUSTOM_ID: exercises-bottom-madness
:END:
Page 325.

*** 01
:PROPERTIES:
:CUSTOM_ID: section-3
:END:
Bottom because each element of the first generator will be applied to
each element of the second generator.

*** 02
:PROPERTIES:
:CUSTOM_ID: section-4
:END:
Produces =[1]= instead of bottom because of laziness and the fact that
=take 1= does not require the list to be evaluated up to =undefined=.

*** 03
:PROPERTIES:
:CUSTOM_ID: section-5
:END:
Bottom because =sum= is strict on the values.

*** 04
:PROPERTIES:
:CUSTOM_ID: section-6
:END:
Works fine because =length= only cares about the spine.

*** 05
:PROPERTIES:
:CUSTOM_ID: section-7
:END:
Because we concatenate the list with =undefined=, it makes part of the
spine, crashing =length=.

*** 06
:PROPERTIES:
:CUSTOM_ID: section-8
:END:
Produces =[2]=. Does not reach =undefined= because of =take 1=.

*** 07
:PROPERTIES:
:CUSTOM_ID: section-9
:END:
We reach =undefined= before finding and even number, causing a crash
(bottom).

*** 08
:PROPERTIES:
:CUSTOM_ID: section-10
:END:
We are able to produce one value before reaching undefined.

*** 09
:PROPERTIES:
:CUSTOM_ID: section-11
:END:
We are able to produce two values before hitting undefined.

*** 10
:PROPERTIES:
:CUSTOM_ID: section-12
:END:
Bottom. Reach undefined before being able to produce three valid values.

* Intermission: Is it in normal form?
:PROPERTIES:
:CUSTOM_ID: intermission-is-it-in-normal-form
:END:
*** 01
:PROPERTIES:
:CUSTOM_ID: section-13
:END:
NF, WHNF.

The list is fully evaluated and all its values are known.

*** 02
:PROPERTIES:
:CUSTOM_ID: section-14
:END:
WHNF.

The list is not fully known because it has the =_= hole.

*** 03
:PROPERTIES:
:CUSTOM_ID: section-15
:END:
Neither. The expression is a function fully applied which has not yet
been evaluated.

*** 04
:PROPERTIES:
:CUSTOM_ID: section-16
:END:
Idem

*** 05
:PROPERTIES:
:CUSTOM_ID: section-17
:END:
Idem

*** 06
:PROPERTIES:
:CUSTOM_ID: section-18
:END:
Idem. =++= is a fully applied function but its operands have not bee
fully evaluated yet.

*** 07
:PROPERTIES:
:CUSTOM_ID: section-19
:END:
WHNF.

It is a data constructor and one of its arguments is still unknown (the
=_=).

* Exercises: More bottoms
:PROPERTIES:
:CUSTOM_ID: exercises-more-bottoms
:END:
Page 332.

*** 01
:PROPERTIES:
:CUSTOM_ID: section-20
:END:
Bottom. We take 1, but the first evaluated element of the list is
'undefined'.

*** 02
:PROPERTIES:
:CUSTOM_ID: section-21
:END:
Produces the value 2. This time, we still take 1, but 'undefined' is the
second element of the list.

*** 03
:PROPERTIES:
:CUSTOM_ID: section-22
:END:
Bottom. We take 2, and 'undefined' appears as the second element of the
list.

*** 04
:PROPERTIES:
:CUSTOM_ID: section-23
:END:
The type signatures means it maps a list of Char to a list of Bool.

It produces a new list of =Bool= . Lowercase vowels are =True=, other
chars, =False=

#+begin_src haskell
f :: [Char] -> [Bool]
f xs = map (\x -> elem x "aeiou") xs
#+end_src

*** 05
:PROPERTIES:
:CUSTOM_ID: section-24
:END:
**** a
:PROPERTIES:
:CUSTOM_ID: a
:END:
Use sectioning for the =^= function so each element of the list is to
the left of the =^=. Takes each element of the list to the power of 2.

#+begin_src ghci
λ> map (^ 2) [1..10]
[1,4,9,16,25,36,49,64,81,100]
#+end_src

**** b
:PROPERTIES:
:CUSTOM_ID: b
:END:
Produces a new list containing the minimum (lowest) value of each inner
list.

#+begin_src ghci
λ> map minimum [[1..10], [10..20], [20..30]]
[1,10,20]
#+end_src

**** c
:PROPERTIES:
:CUSTOM_ID: c
:END:
Produces a list with the sums of each inner list.

#+begin_src ghci
λ> map sum [[1..5], [1..5], [1..5]]
[15,15,15]
#+end_src

*** 06
:PROPERTIES:
:CUSTOM_ID: section-25
:END:
With =bool=, if the third argument is =False=, return the first
argument, otherwise, return the second argument.

#+begin_src ghci
λ> import Data.Bool (bool)
λ> map (\x -> bool (x + 100) (- x) (x == 3)) [1 .. 5]
[101,102,-3,104,105]
#+end_src

* Exercises: Filtering
:PROPERTIES:
:CUSTOM_ID: exercises-filtering
:END:
Page 335.

*** 01
:PROPERTIES:
:CUSTOM_ID: section-26
:END:
#+begin_src ghci
λ> filter (\n -> rem n 3 == 0) [1..30]
[3,6,9,12,15,18,21,24,27,30]

λ> [n | n <- [1..30], rem n 3 == 0]
[3,6,9,12,15,18,21,24,27,30]
#+end_src

*** 02
:PROPERTIES:
:CUSTOM_ID: section-27
:END:
#+begin_src haskell
multOf :: Int -> [Int] -> [Int]
multOf n genList =
  filter (\x -> rem x n == 0) genList

multOf3 :: [Int] -> [Int]
multOf3 = multOf 3

-- OK
r1 = (length . multOf3) [1..30]

-- OK
r2 = (length . multOf 3) [1..30]

-- Oops.
r3 = (length . multOf) 3 [1..30]
#+end_src

Looks like function composition in Haskell does not syntax sugar "one
argument per function" to appear it takes multiple arguments. A composed
chain of functions takes only one argument (unlike Ramda.js, for
example, in which the first function in the chain can take as many
arguments as necessary.)

*** 03
:PROPERTIES:
:CUSTOM_ID: section-28
:END:
#+begin_src haskell
s1 = "the brown dog was a goof"
s2 = "there is an old jedi here"

dropArticles :: [Char] -> [[Char]]
dropArticles s = filter isNotArticle $ words s
  where isNotArticle w = not $ elem w ["a", "an", "the"]
--
-- λ> dropArticles s1
-- ["brown","dog","was","goof"]
-- λ> dropArticles s2
-- ["there","is","old","jedi","here"]
--
#+end_src

* Zipping exercises
:PROPERTIES:
:CUSTOM_ID: zipping-exercises
:END:
Page 337.

*** 01, 02, 03
:PROPERTIES:
:CUSTOM_ID: section-29
:END:
#+begin_src haskell
myZip :: [a] -> [b] -> [(a, b)]
myZip [] _          = []
myZip _  []         = []
myZip (x:xs) (y:ys) = [(x, y)] ++ myZip xs ys

myZipWith :: (a -> b -> c) -> [a] -> [b] -> [c]
myZipWith _ [] _          = []
myZipWith _ _  []         = []
myZipWith f (x:xs) (y:ys) = [f x y] ++ myZipWith f xs ys

myZip' :: [a] -> [b] -> [(a, b)]
myZip' [] _          = []
myZip' _  []         = []
myZip' (x:xs) (y:ys) =
  (myZipWith (,) [x] [y]) ++ myZip' xs ys

myZip'' :: [a] -> [b] -> [(a, b)]
myZip'' [] _          = []
myZip'' _  []         = []
myZip'' xs ys =
  (myZipWith (,) xs ys) ++ myZip'' (tail xs) (tail ys)


myZip''' :: [a] -> [b] -> [(a, b)]
myZip''' [] _  = []
myZip''' _  [] = []
myZip''' xs ys = myZipWith (,) xs ys
#+end_src

TODO: Why can't I simply do:

#+begin_example
myZip' :: [a] -> [b] -> [(a, b)]
myZip' [] _  = []
myZip' _  [] = []
myZip' = myZipWith (,)
#+end_example

Shouldn't it work since partially applying =myZipWith (,)= returns a
function that expect the two remaining lists?

* Chapter Exercises
:PROPERTIES:
:CUSTOM_ID: chapter-exercises
:END:
*** Data.Char
:PROPERTIES:
:CUSTOM_ID: data.char
:END:
Page 338.

Assume this for all the solutions:

#+begin_src haskell
import Data.Char (isUpper, toUpper)
#+end_src

**** 01
:PROPERTIES:
:CUSTOM_ID: section-30
:END:
#+begin_src ghci
λ> :t toUpper
toUpper :: Char -> Char
λ> :t isUpper
isUpper :: Char -> Bool
#+end_src

**** 02
:PROPERTIES:
:CUSTOM_ID: section-31
:END:
Using function composition:

#+begin_src haskell
dropUppers :: [Char] -> [Char]
dropUppers = filter $ not . isUpper

onlyUppers :: [Char] -> [Char]
onlyUppers = filter isUpper
#+end_src

**** 03
:PROPERTIES:
:CUSTOM_ID: section-32
:END:
#+begin_src haskell
capitFst :: [Char] -> [Char]
capitFst str = [toUpper . head $ str] ++ tail str

-- More elegant. Uses pattern-matching, which
-- simplifies the body.
capitFst' :: [Char] -> [Char]
capitFst' (x:xs) = [toUpper x] ++ xs
#+end_src

Or using cons syntax:

#+begin_src haskell
capitalizeFirst :: [Char] -> [Char]
capitalizeFirst []     = []
capitalizeFirst (c:cs) = toUpper c : cs
#+end_src

**** 04
:PROPERTIES:
:CUSTOM_ID: section-33
:END:
#+begin_src haskell
capit :: [Char] -> [Char]
capit [] = []
capit (x:xs) = [toUpper x] ++ capit xs
#+end_src

Or using cons syntax:

#+begin_src hs
capitalizeAll :: [Char] -> [Char]
capitalizeAll []     = []
capitalizeAll (c:cs) = toUpper c : capitalizeAll cs
#+end_src

**** 05, 06
:PROPERTIES:
:CUSTOM_ID: section-34
:END:
#+begin_src haskell
-- The exercise wants us to use ‘head’ instead of
-- pattern-matching on the first cons cell of the spine.

-- Using pattern-matching anyway.
upFst :: [Char] -> Char
upFst (x:_) = toUpper x

upFst' :: [Char] -> Char
upFst' s = toUpper $ head s

upFst'' s = toUpper . head $ s

upFst''' = toUpper . head
#+end_src

*** Ciphers
:PROPERTIES:
:CUSTOM_ID: ciphers
:END:
Page 339.

***** Caesar Solution 1
:PROPERTIES:
:CUSTOM_ID: caesar-solution-1
:END:
Solution from my first study of the book

#+begin_src haskell
{-# LANGUAGE NoMonomorphismRestriction #-}

module Chipher where

import Data.Char

--
-- Where ‘mod’ should wrap around. In this case, it is the
-- length of the alphabet plus 1.
--
wrap :: Int
wrap = ord 'z' - ord 'a' + 1 -- 26

--
-- From an alphabet ranging from 0 to 25, ‘a’ is 0, ‘b’ is
-- 1, ‘z’ is 25.
--
pos :: Char -> Int
pos c = ord c - ord 'a'


rotate :: (Int -> Int -> Int) -> Int -> Char -> Char
rotate _ _ ' ' = ' '
rotate f step c   = newChar
  where
    newPos = mod (pos c `f` step) wrap
    newChar = chr (newPos + ord 'a')


caesar :: Int -> [Char] -> [Char]
caesar step str = map (rotate (-) step) str


unCaesar :: Int -> [Char] -> [Char]
unCaesar step str = map (rotate (+) step) str


orig = "the quick brown fox jumps over the lazy dog"
caesared = "qeb nrfzh yoltk clu grjmp lsbo qeb ixwv ald"


main :: IO ()
main = do
  print $ caesar 3 orig == caesared
  print $ unCaesar 3 caesared == orig
#+end_src

***** Caesar Solution 2
:PROPERTIES:
:CUSTOM_ID: caesar-solution-2
:END:
#+begin_src haskell
{-# LANGUAGE NoMonomorphismRestriction #-}

module Cipher where

--
-- The english alphabet has 26 characters.
--

import Data.Char (chr, ord)

shift :: Int -> Char -> Char
shift step char =
  chr $ (mod (ord char - ai + step) 26) + ai
  where
    ai :: Int
    ai = ord 'a'

caesar :: Int -> [Char] -> [Char]
caesar n = map (shift n)

unCaesar :: Int -> [Char] -> [Char]
unCaesar n = caesar (- n)

--
-- λ> caesar 3 "abc"
-- "def"
--
-- λ> caesar 3 "hello"
-- "khoor"
--
-- λ> unCaesar 3 it
-- "hello"
--
-- λ> caesar 3 "xyz"
-- "abc"
--
-- λ> unCaesar 3 it
-- "xyz"
--
#+end_src

***** Caesar Solution 3
:PROPERTIES:
:CUSTOM_ID: caesar-solution-3
:END:
#+begin_src haskell
{-# LANGUAGE NoMonomorphismRestriction #-}

module Cipher where

--
-- The english alphabet has 26 characters.
--

import Data.Char (chr, ord)

shift :: Int -> Char -> Char
shift step char =
  -- chr $ ai + (mod (pos char + step) 26)
  chr $ move (pos char) step
  where
    ai :: Int
    ai = ord 'a'
    pos :: Char -> Int
    pos c = (ord c - ai)
    move :: Int -> Int -> Int
    move p n = (mod (p + n) 26) + ai

caesar :: Int -> [Char] -> [Char]
caesar n = map (shift n)

unCaesar :: Int -> [Char] -> [Char]
unCaesar n = caesar (- n)

--
-- λ> caesar 3 "abc"
-- "def"
--
-- λ> caesar 3 "hello"
-- "khoor"
--
-- λ> unCaesar 3 it
-- "hello"
--
-- λ> caesar 3 "xyz"
-- "abc"
--
-- λ> unCaesar 3 it
-- "xyz"
--
#+end_src

*** Writing your own standard functions
:PROPERTIES:
:CUSTOM_ID: writing-your-own-standard-functions
:END:
Page 341.

#+begin_src haskell
myAnd :: [Bool] -> Bool
myAnd []     = True
myAnd (x:xs) = x && myAnd xs


myOr :: [Bool] -> Bool
myOr []     = False
myOr (x:xs) = x || myOr xs


myAny :: (a -> Bool) -> [a] -> Bool
myAny _ []     = False
myAny f (x:xs) = f x || myAny f xs


myElem :: Eq a => a -> [a] -> Bool
myElem _ []     = False
myElem e (x:xs) = e == x || myElem e xs


myElem' :: Eq a => a -> [a] -> Bool
myElem' e = myAny (e ==)


myRev :: [a] -> [a]
myRev []     = []
myRev (x:xs) = myRev xs ++ [x]


squish :: [[a]] -> [a]
squish []            = []
squish (xs:listOfXs) = xs ++ squish listOfXs


squishMap :: (a -> [b]) -> [a] -> [b]
squishMap _ []     = []
squishMap f (x:xs) = f x ++ squishMap f xs
--
-- λ> squishMap (\x -> "  __" ++ [x] ++ "__") "abc"
-- "  __a__  __b__  __c__"
--

squishAgain :: [[a]] -> [a]
squishAgain [] = []
squishAgain listOfXs = squishMap (\xs -> xs ++ []) listOfXs
--
-- λ> squishAgain [[1..3], [4..6]]
-- [1,2,3,4,5,6]
--

squishAgainPF :: [[a]] -> [a]
squishAgainPF = squishMap (\xs -> xs ++ [])
--
-- λ> squishAgain [[1..3], [4..6]]
-- [1,2,3,4,5,6]
--


myMaximumBy :: (a -> a -> Ordering) -> [a] -> a
myMaximumBy _ [x] = x
myMaximumBy compFn (x:xs) =
  case compFn x (myMaximumBy compFn xs) of
    GT -> x
    EQ -> x
    LT -> myMaximumBy compFn xs

--
-- Fails with empty list, as does standard `maximumBy`. Version from
-- my second take on the book.
--
myMaximumBy :: (a -> a -> Ordering) -> [a] -> a
myMaximumBy fn list = go fn (tail list) (head list)
  where
    go :: (a -> a -> Ordering) -> [a] -> a -> a
    go _ [] maxSoFar = maxSoFar
    go f (x:xs) maxSoFar =
      case f x maxSoFar of
        GT -> go f xs x -- x is the new maxSoFar
        _  -> go f xs maxSoFar -- maxSoFar is still the maximum so far


myMinimumBy :: (a -> a -> Ordering) -> [a] -> a
myMinimumBy _ [x] = x
myMinimumBy compFn (x:xs) =
  case compFn x (myMinimumBy compFn xs) of
    LT -> x
    EQ -> x
    GT -> myMinimumBy compFn xs

myMininumBy :: (a -> a -> Ordering) -> [a] -> a
myMininumBy fn list = go fn (tail list) (head list)
  where
    go :: (a -> a -> Ordering) -> [a] -> a -> a
    go _ [] minSoFar = minSoFar
    go f (x:xs) minSoFar =
      case f x minSoFar of
        LT -> go f xs x -- x is the new minSoFar
        _  -> go f xs minSoFar -- minSoFar is still the minimum so far

myMaximum :: Ord a => [a] -> a
myMaximum = myMaximumBy compare

myMinimum :: Ord a => [a] -> a
myMinimum = myMinimumBy compare
#+end_src

* The End
:PROPERTIES:
:CUSTOM_ID: the-end
:END:
